// https://www.geeksforgeeks.org/problems/trail-of-ones3242/1

To solve the **"Trail of Ones"** problem optimally, we use a smart **combinatorial trick** based on **Fibonacci numbers**.

---

### ‚úÖ **Problem Summary**

Given `n`, count the number of binary strings of length `n` that contain **at least one pair of consecutive 1's**.

---

### ‚úÖ **Key Insight**

* Total binary strings of length `n`: $2^n$
* Count of binary strings **without** consecutive `1`s is **Fib(n+2)** (Fibonacci trick).

Thus:

> **Answer = 2‚Åø - Fib(n+2)**

---

### ‚úÖ **Why Fib(n+2) for "no consecutive 1's"?**

This is a classic result:

* `dp[i] = dp[i-1] + dp[i-2]`
* You can place a `0`, or place `1` only if previous wasn't `1`.

---

### ‚úÖ Final Java Code (O(n) Time, O(1) Space)

```java
class Solution {
    public int countConsec(int n) {
        int total = 1 << n;  // 2^n
        int fib1 = 1, fib2 = 2;

        for (int i = 3; i <= n + 2; i++) {
            int temp = fib1 + fib2;
            fib1 = fib2;
            fib2 = temp;
        }

        return total - fib2;  // total - Fib(n+2)
    }
}
```

---

### üîç Example:

For `n = 3`:

* Total strings: $2^3 = 8$
* Strings **without** consecutive 1's: Fib(5) = 5 ‚Üí {000, 001, 010, 100, 101}
* So answer = 8 - 5 = **3**

---

### ‚úÖ Time & Space

* **Time:** `O(n)`
* **Space:** `O(1)`

---

### ‚úÖ **Corrected Insight**

We need:

> `count = 2^n - Fib(n+2)`

But in your current code:

* You started `fib1 = 1`, `fib2 = 2`, which gives:

  ```
  Fib(1) = 1  
  Fib(2) = 2  
  Fib(3) = 3  
  ...
  ```

  This is **shifted incorrectly**.

---

### ‚úÖ Proper Fibonacci Base Cases:

We want:

* Fib(0) = 0
* Fib(1) = 1
* Fib(2) = 1
* Fib(3) = 2
* Fib(4) = 3
* Fib(5) = 5

So, we fix base:

```java
int fib0 = 0, fib1 = 1; // Start from Fib(0) and Fib(1)
```

And loop to `Fib(n+2)`

---

### ‚úÖ Final Correct Java Code:

```java
class Solution {
    public int countConsec(int n) {
        int total = 1 << n;  // 2^n
        int fib0 = 0, fib1 = 1, fibN = 0;

        for (int i = 2; i <= n + 2; i++) {
            fibN = fib0 + fib1;
            fib0 = fib1;
            fib1 = fibN;
        }

        return total - fibN;
    }
}
```

---

### üîç Example Fix Check:

For `n = 2`:

* Total: `2^2 = 4`
* Fib(4) = 3
* Ans = `4 - 3 = 1` ‚úÖ
