// https://www.geeksforgeeks.org/problems/lcs-of-three-strings0028/1

Let's solve the **LCS of Three Strings** problem in Java using **bottom-up Dynamic Programming**.

---

### âœ… **Plan (Pseudocode):**

1. Let `s1.length = n1`, `s2.length = n2`, `s3.length = n3`.
2. Create a 3D DP table `dp[n1+1][n2+1][n3+1]` where:

   * `dp[i][j][k]` is the LCS of first `i` chars of `s1`, `j` of `s2`, and `k` of `s3`.
3. Initialize base cases: All zeros when any string is empty.
4. Fill table:

   * If `s1[i-1] == s2[j-1] == s3[k-1]`, then `dp[i][j][k] = 1 + dp[i-1][j-1][k-1]`.
   * Else, `dp[i][j][k] = max(dp[i-1][j][k], dp[i][j-1][k], dp[i][j][k-1])`.

---

### ðŸ’¡ Time and Space Complexity:

* **Time:** O(n1 \* n2 \* n3)
* **Space:** O(n1 \* n2 \* n3) (can optimize with 2 2D arrays, but this is already optimal for clarity and performance)

---

### âœ… Final Java Code:

```java
class Solution {
    public int lcsOf3(String s1, String s2, String s3) {
        int n1 = s1.length(), n2 = s2.length(), n3 = s3.length();
        int[][][] dp = new int[n1 + 1][n2 + 1][n3 + 1];

        for (int i = 1; i <= n1; i++) {
            for (int j = 1; j <= n2; j++) {
                for (int k = 1; k <= n3; k++) {
                    if (s1.charAt(i - 1) == s2.charAt(j - 1) && s2.charAt(j - 1) == s3.charAt(k - 1)) {
                        dp[i][j][k] = 1 + dp[i - 1][j - 1][k - 1];
                    } else {
                        dp[i][j][k] = Math.max(
                            Math.max(dp[i - 1][j][k], dp[i][j - 1][k]),
                            dp[i][j][k - 1]
                        );
                    }
                }
            }
        }
        return dp[n1][n2][n3];
    }
}
```
